FORS_TW_ES.ec
@@ -1,8 +1,9 @@
 (* - Require/Import - *)
 (* -- Built-In (Standard Library) -- *)
-require import AllCore List Distr SmtMap DList FinType IntDiv BitEncoding StdOrder .
+require import AllCore List Distr SmtMap DList FinType IntDiv BitEncoding StdOrder.
 (*---*) import BS2Int BitChunking.
 (*---*) import RealOrder.
+
 
 (* -- Local -- *)
 require import BinaryTrees MerkleTrees.
@@ -2406,7 +2407,7 @@ module (R_TRCOSMDTTCRC_EUFCMA (A : Adv_EUFCMA_MFORSTWESNPRF) : TRCOC_TCR.Adv_SMD
 }.
 
 section Proof_EUFCMA_M_FORS_TW_ES.
-
+print O_ITSR_Default.
 declare module A <: Adv_EUFCMA_MFORSTWESNPRF {-O_CMA_MFORSTWESNPRF, -O_ITSR_Default, -F_OpenPRE.O_SMDTOpenPRE_Default, -FP_OpenPRE.O_SMDTOpenPRE_Default, -FC_TCR.O_SMDTTCR_Default, -TRHC_TCR.O_SMDTTCR_Default, -TRCOC_TCR.O_SMDTTCR_Default, -O_THFC_Default, -R_ITSR_EUFCMA, -R_FSMDTOpenPRE_EUFCMA, -R_TRHSMDTTCRC_EUFCMA, -R_TRCOSMDTTCRC_EUFCMA}.
 
 (* As EUF_CMA_MFORSTWESNPRF, but with additional checks for possibility of breaking considered properties of THFs  *)
@@ -2641,8 +2642,8 @@ seq 4 4 : (   ={pp, i}
     while (   ={tws_init}
            /\ size tws_init{1} = d * k * t
            /\ ys0{1} = ys1{2}
-           /\ ={pp, ts}(O_SMDTOpenPRE_Default, FP_OpenPRE.O_SMDTOpenPRE_Default) /\
-    O_SMDTOpenPRE_Default.xs{1} = map DigestBlock.val FP_OpenPRE.O_SMDTOpenPRE_Default.xs{2}
+           /\ ={pp, ts}(O_SMDTOpenPRE_Default, FP_OpenPRE.O_SMDTOpenPRE_Default) 
+           /\ O_SMDTOpenPRE_Default.xs{1} = map DigestBlock.val FP_OpenPRE.O_SMDTOpenPRE_Default.xs{2}
            /\ size FP_OpenPRE.O_SMDTOpenPRE_Default.xs{2} = size FP_OpenPRE.O_SMDTOpenPRE_Default.ts{2}
            /\ size FP_OpenPRE.O_SMDTOpenPRE_Default.ts{2} <= min (size tws_init{2}) (d * k * t)).
     * wp; rnd DigestBlock.insubd DigestBlock.val.
